Introduce value preservation lemma 15.9 from the spec

Isabelle/Shelley/Delegation.thy
@@ -8,7 +8,11 @@ subsection \<open> Delegation Transitions \<close>
 
 text \<open> Delegation States \<close>
 
-type_synonym d_state = "(addr_rwd, coin) fmap" \<comment> \<open>NOTE: Only rewards for now\<close>
+\<comment> \<open>NOTE: Only \<open>stkCreds\<close>, \<open>rewards\<close> and \<open>i\<^sub>r\<^sub>w\<^sub>d\<close> for now\<close>
+type_synonym d_state = "
+  stake_creds \<times> \<comment> \<open>registered stake delegators\<close>
+  (addr_rwd, coin) fmap \<times> \<comment> \<open>rewards\<close>
+  (credential, coin) fmap \<comment> \<open>instantaneous rewards\<close>"
 
 typedecl p_state \<comment> \<open>NOTE: Abstract for now\<close>
 
@@ -28,19 +32,26 @@ text \<open>
   precondition \<open>addr_rwd hk \<notin> dom rewards\<close> or use \<open>\<union>\<^sub>\<leftarrow>\<close> instead of \<open>++\<^sub>f\<close> in rule \<open>deleg_reg\<close> since
   Lemma 15.6 is a property of \<open>DELEG\<close>.
  \<close>
-
 inductive deleg_sts :: "d_env \<Rightarrow> d_state \<Rightarrow> d_cert \<Rightarrow> d_state \<Rightarrow> bool"
   (\<open>_ \<turnstile> _ \<rightarrow>\<^bsub>DELEG\<^esub>{_} _\<close> [51, 0, 51] 50)
   where
     deleg_reg: "
-      \<Gamma> \<turnstile> rewards \<rightarrow>\<^bsub>DELEG\<^esub>{c} rewards \<union>\<^sub>\<leftarrow> {addr_rwd hk $$:= 0}"
+      slot \<turnstile>
+        (stk_creds, rewards, i\<^sub>r\<^sub>w\<^sub>d)
+          \<rightarrow>\<^bsub>DELEG\<^esub>{c}
+        (stk_creds ++\<^sub>f {hk $$:= slot}, rewards \<union>\<^sub>\<leftarrow> {addr_rwd hk $$:= 0}, i\<^sub>r\<^sub>w\<^sub>d)"
       if "c = DCert_RegKey"
       and "hk = reg_cred c"
+      and "hk \<notin> fmdom' stk_creds"
   | deleg_dereg: "
-      \<Gamma> \<turnstile> rewards \<rightarrow>\<^bsub>DELEG\<^esub>{c} {addr_rwd hk} \<lhd>/ rewards"
+      slot \<turnstile>
+        (stk_creds, rewards, i\<^sub>r\<^sub>w\<^sub>d)
+          \<rightarrow>\<^bsub>DELEG\<^esub>{c}
+        ({hk} \<lhd>/ stk_creds, {addr_rwd hk} \<lhd>/ rewards, i\<^sub>r\<^sub>w\<^sub>d)"
       if "c = DCert_DeregKey"
       and "hk = cwitness c"
       and "rewards $$ (addr_rwd hk) = Some 0"
+      and "hk \<in> fmdom' stk_creds"
 
 subsection \<open> Delegation and Pool Combined Rules \<close>
 
@@ -79,7 +90,8 @@ inductive delegs_sts :: "d_p_s_env \<Rightarrow> d_p_state \<Rightarrow> d_cert 
   (\<open>_ \<turnstile> _ \<rightarrow>\<^bsub>DELEGS\<^esub>{_} _\<close> [51, 0, 51] 50)
   where
     seq_delg_base: "
-      (slot, tx) \<turnstile> (rewards, pstate) \<rightarrow>\<^bsub>DELEGS\<^esub>{[]} (rewards', pstate)"
+      (slot, tx) \<turnstile>
+        ((stk_creds, rewards, i\<^sub>r\<^sub>w\<^sub>d), pstate) \<rightarrow>\<^bsub>DELEGS\<^esub>{[]} ((stk_creds, rewards', i\<^sub>r\<^sub>w\<^sub>d), pstate)"
       if "wdrls = txwdrls tx"
       and "wdrls \<subseteq>\<^sub>f rewards"
       and "rewards' = rewards \<union>\<^sub>\<rightarrow> fmmap (\<lambda>_. 0) wdrls"
