Isabelle/Shelley/Rewards.thy
@@ -1,6 +1,7 @@
 section \<open> Rewards and the Epoch Boundary \<close>
+
 theory Rewards
-  imports UTxO Delegation Protocol_Parameters
+  imports UTxO Delegation Protocol_Parameters Ledger
 begin
 
 subsection \<open> Helper Functions and Accounting Fields \<close>
@@ -8,6 +9,27 @@ subsection \<open> Helper Functions and Accounting Fields \<close>
 text \<open> Accounting Fields \<close>
 
 type_synonym acnt = "coin \<times> coin"
+
+subsection \<open> Stake Distribution Calculation \<close>
+
+text \<open> Blocks made by stake pools \<close>
+
+type_synonym blocks_made = "(key_hash, nat) fmap"
+
+text \<open> Stake \<close>
+
+type_synonym stake = "(key_hash, coin) fmap"
+
+subsection \<open> Snapshot Transition \<close>
+
+text \<open> Snapshots \<close>
+
+type_synonym snapshots = "
+  (stake \<times> (key_hash, key_hash) fmap) \<times> \<comment> \<open>newest stake\<close>
+  (stake \<times> (key_hash, key_hash) fmap) \<times> \<comment> \<open>middle stake\<close>
+  (stake \<times> (key_hash, key_hash) fmap) \<times> \<comment> \<open>oldest stake\<close>
+  (key_hash, pool_param) fmap \<times> \<comment> \<open>pool parameters\<close>
+  coin \<comment> \<open>fee snapshot\<close>"
 
 subsection \<open> Pool Reaping Transition \<close>
 
@@ -29,14 +51,14 @@ inductive poolreap_sts :: "p_params \<Rightarrow> pl_reap_state \<Rightarrow> ep
         (
           (utxo, deps, fees, ups),
           (treasury, reserves),
-          rewards,
+          (stk_creds, rewards, i\<^sub>r\<^sub>w\<^sub>d),
           pstate
         )
          \<rightarrow>\<^bsub>POOLREAP\<^esub>{e}
         (
           (utxo, deps - (unclaimed + refunded), fees, ups),
           (treasury + unclaimed, reserves),
-          rewards \<union>\<^sub>+ refunds,
+          (stk_creds, rewards \<union>\<^sub>+ refunds, i\<^sub>r\<^sub>w\<^sub>d),
           pstate
         )"
       if "reward_acnts' = undefined"
@@ -44,5 +66,86 @@ inductive poolreap_sts :: "p_params \<Rightarrow> pl_reap_state \<Rightarrow> ep
       and "m_refunds = fmdom' rewards \<lhd>/ reward_acnts'"
       and "refunded = (\<Sum>k \<in> fmdom' refunds. refunds $$! k)"
       and "unclaimed = (\<Sum>k \<in> fmdom' m_refunds. m_refunds $$! k)"
+
+subsection \<open> Complete Epoch Boundary Transition \<close>
+
+text \<open> Epoch States \<close>
+
+type_synonym epoch_state = "acnt \<times> snapshots \<times> l_state \<times> p_params"
+
+subsection \<open> Reward Distribution Calculation \<close>
+
+text \<open> Calculation to reward all stake pools \<close>
+
+fun reward :: "p_params \<Rightarrow> blocks_made \<Rightarrow> coin \<Rightarrow> addr_rwd set \<Rightarrow> (key_hash, pool_param) fmap \<Rightarrow>
+  stake \<Rightarrow> (key_hash, key_hash) fmap \<Rightarrow> (addr_rwd, coin) fmap" where
+  "reward pp blocks R addrs\<^sub>r\<^sub>e\<^sub>w pool_params stake delegs = undefined" \<comment> \<open>NOTE: Undefined for now\<close>
+
+subsection \<open> Reward Update Calculation \<close>
+
+text \<open> Reward Update \<close>
+
+type_synonym reward_update = "coin \<times> coin \<times> (addr_rwd, coin) fmap \<times> coin \<times> (credential, coin) fmap"
+
+text \<open> Calculation to create a reward update \<close>
+
+fun create_r_upd :: "blocks_made \<Rightarrow> epoch_state \<Rightarrow> reward_update" where
+  "create_r_upd b
+    (
+      (_, reserves),
+      (_, _, (stake, delegs), pools_ss, fee_ss),
+      (_, ((stk_creds, rewards, i\<^sub>r\<^sub>w\<^sub>d), _)),
+      pp
+    ) =
+    (
+      let
+        unregistered = fmdom' stk_creds \<lhd>/ i\<^sub>r\<^sub>w\<^sub>d;
+        registered = i\<^sub>r\<^sub>w\<^sub>d --\<^sub>f unregistered;
+        rewards\<^sub>m\<^sub>i\<^sub>r = (\<Sum> k \<in> fmdom' registered. registered $$! k);
+        reserves' = reserves - rewards\<^sub>m\<^sub>i\<^sub>r;
+        blocks_made = (\<Sum> k \<in> fmdom' b. b $$! k);
+        \<eta> = real blocks_made / (real slots_per_epoch * active_slot_coeff pp);
+        \<Delta>r\<^sub>l = \<lfloor>min 1 \<eta> * rho pp * reserves'\<rfloor>;
+        reward_pot = fee_ss + \<Delta>r\<^sub>l;
+        \<Delta>t\<^sub>1 = \<lfloor>tau pp * reward_pot\<rfloor>;
+        \<Delta>r = \<Delta>r\<^sub>l + rewards\<^sub>m\<^sub>i\<^sub>r;
+        R = reward_pot - \<Delta>t\<^sub>1;
+        rs = reward pp b R (fmdom' rewards) pools_ss stake delegs;
+        \<Delta>t\<^sub>2 = R - (\<Sum> k \<in> fmdom' rs. rs $$! k)
+      in
+        (\<Delta>t\<^sub>1 + \<Delta>t\<^sub>2, -\<Delta>r, rs, -fee_ss, registered)
+    )"
+
+text \<open> Applying a reward update \<close>
+
+fun apply_r_upd :: "reward_update \<Rightarrow> epoch_state \<Rightarrow> epoch_state" where
+  "apply_r_upd
+    (\<Delta>t, \<Delta>r, rs, \<Delta>f, rew\<^sub>m\<^sub>i\<^sub>r)
+    (
+      (treasury, reserves),
+      ss,
+      (
+        (utxo, deps, fees, up),
+        ((stk_creds, rewards, i\<^sub>r\<^sub>w\<^sub>d), pstate)
+      ),
+      ppm
+    ) =
+    (
+      let
+        rew'\<^sub>m\<^sub>i\<^sub>r = fmdom' stk_creds \<lhd> rew\<^sub>m\<^sub>i\<^sub>r;
+        unregistered = fmdom' stk_creds \<lhd>/ rew\<^sub>m\<^sub>i\<^sub>r;
+        non_distributed = (\<Sum>k \<in> fmdom' unregistered. unregistered $$! k);
+        update\<^sub>r\<^sub>w\<^sub>d = fmap_of_list [(addr_rwd hk, val). (hk, val) \<leftarrow> sorted_list_of_fmap rew'\<^sub>m\<^sub>i\<^sub>r]
+      in
+        (
+          (treasury + \<Delta>t, reserves + \<Delta>r + non_distributed),
+          ss,
+          (
+            (utxo, deps, fees + \<Delta>f, up),
+            ((stk_creds, (rewards \<union>\<^sub>+ rs) \<union>\<^sub>+ update\<^sub>r\<^sub>w\<^sub>d, {$$}), pstate)
+          ),
+          ppm
+        )
+    )"
 
 end
