Isabelle/Shelley/Address.thy
@@ -7,6 +7,8 @@ begin
 text \<open> Credential \<close>
 
 typedecl credential \<comment> \<open>NOTE: Abstract for now\<close>
+axiomatization where credential_linorder: "OFCLASS(credential, linorder_class)"
+instance credential :: linorder by (rule credential_linorder)
 
 text \<open> Output address \<close>
 
@@ -15,6 +17,8 @@ typedecl addr \<comment> \<open>NOTE: Abstract for now\<close>
 text \<open> Reward account \<close>
 
 typedecl addr_rwd \<comment> \<open>NOTE: Abstract for now\<close>
+axiomatization where addr_rwd_linorder: "OFCLASS(addr_rwd, linorder_class)"
+instance addr_rwd :: linorder by (rule addr_rwd_linorder)
 
 text \<open> Construct a reward account \<close>
 
