Isabelle/Shelley/Delegation_Certificates.thy
@@ -1,7 +1,7 @@
 section \<open> Delegation certificates \<close>
 
 theory Delegation_Certificates
-  imports Address
+  imports Address Basic_Types Finite_Map_Extras
 begin
 
 subsection \<open> Delegation Definitions \<close>
@@ -12,11 +12,15 @@ datatype d_cert = DCert_RegKey | DCert_DeregKey \<comment> \<open>NOTE: Incomple
 
 text \<open> Registered stake credential \<close>
 
-typedecl stake_creds \<comment> \<open>NOTE: Abstract for now\<close>
+type_synonym stake_creds = "(credential, slot) fmap"
 
 text \<open> Registered stake pools \<close>
 
 typedecl stake_pools \<comment> \<open>NOTE: Abstract for now\<close>
+
+text \<open> Stake pools parameters \<close>
+
+typedecl pool_param \<comment> \<open>NOTE: Abstract for now\<close>
 
 text \<open> Certificate witness \<close>
 
