Isabelle/Shelley/Finite_Map_Extras.thy
@@ -102,8 +102,7 @@ next
   qed
 qed
 
-(* TODO: Find a nicer proof *)
-lemma fmran_singleton: "fmran {k $$:= v} = {|v|}"
+lemma fmran_singleton: "fmran {k $$:= v} = {|v|}" (* TODO: Find a nicer proof *)
 proof -
   have "\<And>v'. v' |\<in>| fmran {k $$:= v} \<Longrightarrow> v' = v"
     by (metis fmdom_empty fmdom_fmupd fmdom_notD fmranE fmupd_lookup fsingleton_iff
@@ -114,14 +113,236 @@ proof -
     by (simp add: fsubsetI fsubset_antisym)
 qed
 
+lemma fmmap_keys_hom:
+  assumes "fmdom' m\<^sub>1 \<inter> fmdom' m\<^sub>2 = {}"
+  shows "fmmap_keys f (m\<^sub>1 ++\<^sub>f m\<^sub>2) = fmmap_keys f m\<^sub>1 ++\<^sub>f fmmap_keys f m\<^sub>2"
+  using assms
+  by (simp add: fmap_ext)
+
+lemma map_insort_is_insort_key:
+  assumes "m $$ k = None"
+  shows "map (\<lambda>k'. (k', m(k $$:= v) $$! k')) (insort k xs) =
+    insort_key fst (k, v) (map (\<lambda>k'. (k', m(k $$:= v) $$! k')) xs)"
+  using assms by (induction xs) auto
+
+lemma sorted_list_of_fmap_is_insort_key_fst:
+  assumes "m $$ k = None"
+  shows "sorted_list_of_fmap m(k $$:= v) = insort_key fst (k, v) (sorted_list_of_fmap m)"
+proof -
+  have "sorted_list_of_fmap m(k $$:= v) =
+    map (\<lambda>k'. (k', m(k $$:= v) $$! k')) (sorted_list_of_fset (fmdom (m(k $$:= v))))"
+    unfolding sorted_list_of_fmap_def ..
+  also have "\<dots> = 	map (\<lambda>k'. (k', m(k $$:= v) $$! k')) (sorted_list_of_fset (finsert k (fmdom m)))"
+    by simp
+  also from \<open>m $$ k = None\<close> have "\<dots> =
+    map (\<lambda>k'. (k', m(k $$:= v) $$! k')) (insort k (sorted_list_of_fset (fmdom m - {|k|})))"
+    by (simp add: sorted_list_of_fset.rep_eq)
+  also from \<open>m $$ k = None\<close> have "\<dots> =
+    map (\<lambda>k'. (k', m(k $$:= v) $$! k')) (insort k (sorted_list_of_fset (fmdom m)))"
+    by (simp add: fmdom_notI)
+  also from \<open>m $$ k = None\<close> have "\<dots> =
+    insort_key fst (k, v) (map (\<lambda>k'. (k', m(k $$:= v) $$! k')) (sorted_list_of_fset (fmdom m)))"
+    using map_insort_is_insort_key by fastforce
+  also have "\<dots> = insort_key fst (k, v) (map (\<lambda>k'. (k', m $$! k')) (sorted_list_of_fset (fmdom m)))"
+  proof -
+    from \<open>m $$ k = None\<close> have "\<And>k'. k' \<in> fmdom' m \<Longrightarrow> m(k $$:= v) $$! k' = m $$! k'"
+      using fmdom'_notI by force
+    moreover from \<open>m $$ k = None\<close> have "k \<notin> set (sorted_list_of_fset (fmdom m))"
+      using fmdom'_alt_def and fmdom'_notI and in_set_member by force
+    ultimately show ?thesis
+      by (metis (mono_tags, lifting) fmdom'_alt_def map_eq_conv sorted_list_of_fset_simps(1))
+  qed
+  finally show ?thesis
+    by (simp add: sorted_list_of_fmap_def)
+qed
+
+lemma distinct_fst_inj:
+  assumes "distinct (map fst ps)"
+  and "inj f"
+  shows "distinct (map fst (map (\<lambda>(k, v). (f k, v)) ps))"
+proof -
+  have "map fst (map (\<lambda>(k, v). (f k, v)) ps) = map f (map fst ps)"
+    by (induction ps) auto
+  moreover from assms have "distinct (map f (map fst ps))"
+    by (simp add: distinct_map inj_on_def)
+  ultimately show ?thesis
+    by presburger
+qed
+
+lemma distinct_sorted_list_of_fmap:
+  shows "distinct (map fst (sorted_list_of_fmap m))"
+  unfolding sorted_list_of_fmap_def and sorted_list_of_fset_def
+  by (simp add: distinct_map inj_on_def)
+
+lemma map_inj_pair_non_membership:
+  assumes "k \<notin> set (map fst ps)"
+  and "inj f"
+  shows "f k \<notin> set (map fst (map (\<lambda>(k, v). (f k, v)) ps))"
+  using assms by (induction ps) (simp add: member_rec(2), fastforce simp add: injD)
+
+lemma map_insort_key_fst:
+  assumes "distinct (map fst ps)"
+  and "k \<notin> set (map fst ps)"
+  and "inj f"
+  and "mono f"
+  shows "map (\<lambda>(k, v). (f k, v)) (insort_key fst (k, v) ps) =
+    insort_key fst (f k, v) (map (\<lambda>(k, v). (f k, v)) ps)"
+  using assms
+proof (induction ps)
+  case Nil
+  then show ?case
+    by simp
+next
+  let ?g = "(\<lambda>(k, v). (f k, v))"
+  case (Cons p ps)
+  then show ?case
+  proof (cases "k \<le> fst p")
+    case True
+    let ?f_p = "(f (fst p), snd p)"
+    have "insort_key fst (f k, v) (map ?g (p # ps)) = insort_key fst (f k, v) (?f_p # map ?g ps)"
+      by (simp add: prod.case_eq_if)
+    moreover from Cons.prems(4) and True have "f k \<le> f (fst p)"
+      by (auto dest: monoE)
+    then have "insort_key fst (f k, v) (?f_p # map ?g ps) = (f k, v) # ?f_p # map ?g ps"
+      by simp
+    ultimately have "insort_key fst (f k, v) (map ?g (p # ps)) = (f k, v) # ?f_p # map ?g ps"
+      by simp
+    moreover from True have "map ?g (insort_key fst (k, v) (p # ps)) = (f k, v) # ?f_p # map ?g ps"
+      by (simp add: case_prod_beta')
+    ultimately show ?thesis
+      by simp
+  next
+    case False
+    let ?f_p = "(f (fst p), snd p)"
+    have "insort_key fst (f k, v) (map ?g (p # ps)) = insort_key fst (f k, v) (?f_p # map ?g ps)"
+      by (simp add: prod.case_eq_if)
+    moreover from \<open>mono f\<close> and False have "f (fst p) \<le> f k"
+      using not_le by (blast dest: mono_invE)
+    ultimately have "insort_key fst (f k, v) (map ?g (p # ps)) =
+      ?f_p # insort_key fst (f k, v) (map ?g ps)"
+      using False and \<open>inj f\<close> by (fastforce dest: injD)
+    also from Cons.IH and Cons.prems(1,2) and assms(3,4) have "\<dots> =
+      ?f_p # (map ?g (insort_key fst (k, v) ps))"
+      by (fastforce simp add: member_rec(1))
+    also have "\<dots> = map ?g (p # insort_key fst (k, v) ps)"
+      by (simp add: case_prod_beta)
+    finally show ?thesis
+      using False by simp
+  qed
+qed
+
+lemma map_sorted_list_of_fmap:
+  assumes "inj f"
+  and "mono f"
+  and "m $$ k = None"
+  shows "map (\<lambda>(k, v). (f k, v)) (sorted_list_of_fmap m(k $$:= v)) =
+    insort_key fst (f k, v) (map (\<lambda>(k, v). (f k, v)) (sorted_list_of_fmap m))"
+proof -
+  let ?g = "(\<lambda>(k, v). (f k, v))"
+  from \<open>m $$ k = None\<close> have "map ?g (sorted_list_of_fmap m(k $$:= v)) =
+  	map ?g (insort_key fst (k, v) (sorted_list_of_fmap m))"
+  	using sorted_list_of_fmap_is_insort_key_fst by fastforce
+  also have "\<dots> = insort_key fst (f k, v) (map ?g (sorted_list_of_fmap m))"
+  proof -
+    have "distinct (map fst (sorted_list_of_fmap m))"
+      by (simp add: distinct_sorted_list_of_fmap)
+    moreover from \<open>m $$ k = None\<close> have "k \<notin> set (map fst (sorted_list_of_fmap m))"
+      by (metis image_set map_of_eq_None_iff map_of_sorted_list)
+    ultimately show ?thesis
+      by (simp add: map_insort_key_fst assms(1,2))
+  qed
+  finally show ?thesis .
+qed
+
+lemma fmap_of_list_insort_key_fst:
+  assumes "distinct (map fst ps)"
+  and "k \<notin> set (map fst ps)"
+  shows "fmap_of_list (insort_key fst (k, v) ps) = (fmap_of_list ps)(k $$:= v)"
+  using assms
+proof (induction ps)
+  case Nil
+  then show ?case
+    by simp
+next
+  case (Cons p ps)
+  then show ?case
+  proof (cases "k \<le> fst p")
+    case True
+    then show ?thesis
+      by simp
+  next
+    case False
+    then have "fmap_of_list (insort_key fst (k, v) (p # ps)) =
+      fmap_of_list (p # insort_key fst (k, v) ps)"
+      by simp
+    also have "\<dots> = (fmap_of_list (insort_key fst (k, v) ps))(fst p $$:= snd p)"
+      by (metis fmap_of_list_simps(2) prod.collapse)
+    also from Cons.prems(1,2) and Cons.IH have "\<dots> = (fmap_of_list ps)(k $$:= v)(fst p $$:= snd p)"
+      by (fastforce simp add: member_rec(1))
+    finally show ?thesis
+    proof -
+      assume *: "fmap_of_list (insort_key fst (k, v) (p # ps)) =
+        (fmap_of_list ps)(k $$:= v)(fst p $$:= snd p)"
+      from Cons.prems(2) have "k \<notin> set (fst p # map fst ps)"
+        by simp
+      then have **: "{k $$:= v} $$ (fst p) = None"
+        by (fastforce simp add: member_rec(1))
+      have "fmap_of_list (p # ps) = (fmap_of_list ps)(fst p $$:= snd p)"
+        by (metis fmap_of_list_simps(2) prod.collapse)
+      with * and ** show ?thesis
+        using fmap_singleton_comm by (metis fmadd_fmupd fmap_of_list_simps(1,2) fmupd_alt_def)
+    qed
+  qed
+qed
+
+lemma fmap_of_list_insort_key_fst_map:
+  assumes "inj f"
+  and "m $$ k = None"
+  shows "fmap_of_list (insort_key fst (f k, v) (map (\<lambda>(k, v). (f k, v)) (sorted_list_of_fmap m))) =
+    (fmap_of_list (map (\<lambda>(k, v). (f k, v)) (sorted_list_of_fmap m)))(f k $$:= v)"
+proof -
+  let ?g = "\<lambda>(k, v). (f k, v)"
+  let ?ps = "map ?g (sorted_list_of_fmap m)"
+  from \<open>inj f\<close> have "distinct (map fst ?ps)"
+    using distinct_fst_inj and distinct_sorted_list_of_fmap by fastforce
+  moreover have "f k \<notin> set (map fst ?ps)"
+  proof -
+    from \<open>m $$ k = None\<close> have "k \<notin> set (map fst (sorted_list_of_fmap m))"
+      by (metis map_of_eq_None_iff map_of_sorted_list set_map)
+    with \<open>inj f\<close> show ?thesis
+      using map_inj_pair_non_membership by force
+  qed
+  ultimately show ?thesis
+    using fmap_of_list_insort_key_fst by fast
+qed
+
+lemma fmap_of_list_sorted_list_of_fmap:
+  fixes m :: "('a::linorder, 'b) fmap"
+  and f :: "'a \<Rightarrow> 'c::linorder"
+  assumes "inj f"
+  and "mono f"
+  and "m $$ k = None"
+  shows "fmap_of_list (map (\<lambda>(k, v). (f k, v)) (sorted_list_of_fmap m(k $$:= v))) =
+    (fmap_of_list (map (\<lambda>(k, v). (f k, v)) (sorted_list_of_fmap m)))(f k $$:= v)"
+proof -
+  let ?g = "\<lambda>(k, v). (f k, v)"
+  from assms(3) have "fmap_of_list (map ?g (sorted_list_of_fmap m(k $$:= v))) =
+    fmap_of_list (map ?g (insort_key fst (k, v) (sorted_list_of_fmap m)))"
+    by (simp add: sorted_list_of_fmap_is_insort_key_fst)
+  also from assms have "\<dots> = fmap_of_list (insort_key fst (f k, v) (map ?g (sorted_list_of_fmap m)))"
+    using calculation and map_sorted_list_of_fmap by fastforce
+  also from assms(1,3) have "\<dots> = (fmap_of_list (map ?g (sorted_list_of_fmap m)))(f k $$:= v)"
+    by (simp add: fmap_of_list_insort_key_fst_map)
+  finally show ?thesis .
+qed
+
 text \<open> Map difference \<close>
 
 abbreviation
   fmdiff :: "('a, 'b) fmap \<Rightarrow> ('a, 'b) fmap \<Rightarrow> ('a, 'b) fmap" (infixl \<open>--\<^sub>f\<close> 100) where
   "m\<^sub>1 --\<^sub>f m\<^sub>2 \<equiv> fmfilter (\<lambda>x. x \<notin> fmdom' m\<^sub>2) m\<^sub>1"
 
-(* TODO: Find a nicer proof *)
-lemma fmdiff_partition:
+lemma fmdiff_partition: (* TODO: Find a nicer proof *)
   assumes "m\<^sub>2 \<subseteq>\<^sub>f m\<^sub>1"
   shows "m\<^sub>2 ++\<^sub>f (m\<^sub>1 --\<^sub>f m\<^sub>2) = m\<^sub>1"
 proof -
@@ -133,8 +354,7 @@ proof -
     by (metis (no_types, lifting) domIff fmap_ext fmsubset.rep_eq map_le_def)
 qed
 
-(* TODO: Find a nicer proof *)
-lemma fmdiff_fmupd:
+lemma fmdiff_fmupd: (* TODO: Find a nicer proof *)
   assumes "m $$ k = None"
   shows "m(k $$:= v) --\<^sub>f {k $$:= v} = m"
   using assms
@@ -143,7 +363,7 @@ lemma fmdiff_fmupd:
 
 text \<open> Map symmetric difference \<close>
 
-abbreviation fmsym_diff :: "('a, 'b) fmap \<Rightarrow> ('a, 'b) fmap \<Rightarrow> ('a, 'b) fmap" (infixl "\<Delta>\<^sub>f" 100) where
+abbreviation fmsym_diff :: "('a, 'b) fmap \<Rightarrow> ('a, 'b) fmap \<Rightarrow> ('a, 'b) fmap" (infixl \<open>\<Delta>\<^sub>f\<close> 100) where
   "m\<^sub>1 \<Delta>\<^sub>f m\<^sub>2 \<equiv> (m\<^sub>1 --\<^sub>f m\<^sub>2) ++\<^sub>f (m\<^sub>2 --\<^sub>f m\<^sub>1)"
 
 text \<open> Domain restriction \<close>
@@ -159,7 +379,7 @@ abbreviation dom_exc :: "'a set \<Rightarrow> ('a, 'b) fmap \<Rightarrow> ('a, '
 text \<open> Intersection plus \<close>
 
 abbreviation intersection_plus :: "('a, 'b::monoid_add) fmap \<Rightarrow> ('a, 'b) fmap \<Rightarrow> ('a, 'b) fmap"
-  (infixl "\<inter>\<^sub>+" 100)
+  (infixl \<open>\<inter>\<^sub>+\<close> 100)
 where
   "m\<^sub>1 \<inter>\<^sub>+ m\<^sub>2 \<equiv> fmmap_keys (\<lambda>k v. v + m\<^sub>1 $$! k) (fmdom' m\<^sub>1 \<lhd> m\<^sub>2)"
 
@@ -184,7 +404,7 @@ abbreviation union_override_plus :: "('a, 'b::monoid_add) fmap \<Rightarrow> ('a
 where
   "m\<^sub>1 \<union>\<^sub>+ m\<^sub>2 \<equiv> (m\<^sub>1 \<Delta>\<^sub>f m\<^sub>2) ++\<^sub>f (m\<^sub>1 \<inter>\<^sub>+ m\<^sub>2)"
 
-text \<open> Extra lemmas for \<open>\<lhd>\<close> and \<open>\<lhd>/\<close> \<close>
+text \<open> Extra lemmas for the non-standard map operators \<close>
 
 lemma dom_res_singleton:
   assumes "m $$ k = Some v"
@@ -218,8 +438,7 @@ next
   qed
 qed
 
-(* TODO: Find a nicer proof *)
-lemma dom_res_union_distr:
+lemma dom_res_union_distr: (* TODO: Find a nicer proof *)
   shows "(A \<union> B) \<lhd> m = A \<lhd> m ++\<^sub>f B \<lhd> m"
 proof -
   have "(A \<union> B) \<lhd> m \<subseteq>\<^sub>f A \<lhd> m ++\<^sub>f B \<lhd> m"
@@ -276,6 +495,83 @@ next
     finally show ?thesis
       by auto
   qed
+qed
+
+lemma dom_res_addition_in:
+  assumes "m\<^sub>1 $$ k = None"
+  and "m\<^sub>2 $$ k = Some v'"
+  shows "fmdom' m\<^sub>1(k $$:= v) \<lhd> m\<^sub>2 = fmdom' m\<^sub>1 \<lhd> m\<^sub>2 ++\<^sub>f {k $$:= v'}"
+proof -
+  from \<open>m\<^sub>1 $$ k = None\<close> have "fmdom' m\<^sub>1(k $$:= v) \<lhd> m\<^sub>2 = (fmdom' m\<^sub>1 \<union> {k}) \<lhd> m\<^sub>2"
+    by simp
+  also have "\<dots> = fmdom' m\<^sub>1 \<lhd> m\<^sub>2 ++\<^sub>f {k} \<lhd> m\<^sub>2"
+    using dom_res_union_distr .
+  finally show ?thesis
+    using \<open>m\<^sub>2 $$ k = Some v'\<close> and dom_res_singleton by fastforce
+qed
+
+lemma inter_plus_addition_in: (* TODO: Find nicer proofs for SMT calls. *)
+  assumes "m\<^sub>1 $$ k = None"
+  and "m\<^sub>2 $$ k = Some v'"
+  shows "m\<^sub>1(k $$:= v) \<inter>\<^sub>+ m\<^sub>2 = (m\<^sub>1 \<inter>\<^sub>+ m\<^sub>2) ++\<^sub>f {k $$:= v' + v}"
+proof -
+  from assms have "m\<^sub>1(k $$:= v) \<inter>\<^sub>+ m\<^sub>2 =
+    fmmap_keys (\<lambda>k' v'. v' + m\<^sub>1(k $$:= v) $$! k') ((fmdom' m\<^sub>1 \<lhd> m\<^sub>2) ++\<^sub>f {k $$:= v'})"
+    using dom_res_addition_in by fastforce
+  also have "\<dots> = fmmap_keys (\<lambda>k' v'. v' + m\<^sub>1(k $$:= v) $$! k') (fmdom' m\<^sub>1 \<lhd> m\<^sub>2)
+    ++\<^sub>f fmmap_keys (\<lambda>k' v'. v' + m\<^sub>1(k $$:= v) $$! k') {k $$:= v'}"
+  proof -
+    from \<open>m\<^sub>1 $$ k = None\<close> have "fmdom' (fmdom' m\<^sub>1 \<lhd> m\<^sub>2) \<inter> fmdom' {k $$:= v'} = {}"
+      by (simp add: fmdom'_notI)
+    then show ?thesis
+      using fmmap_keys_hom by blast
+  qed
+  also from assms
+  have "\<dots> = fmmap_keys (\<lambda>k' v'. v' + m\<^sub>1(k $$:= v) $$! k') (fmdom' m\<^sub>1 \<lhd> m\<^sub>2) ++\<^sub>f {k $$:= v' + v}"
+    using dom_res_singleton by (smt domIff dom_fmlookup fmfilter_fmmap_keys fmlookup_dom'_iff
+      fmlookup_fmmap_keys fmupd_lookup map_option_is_None option.map_sel option.sel)
+  also have "\<dots> = fmmap_keys (\<lambda>k' v'. v' + m\<^sub>1 $$! k') (fmdom' m\<^sub>1 \<lhd> m\<^sub>2) ++\<^sub>f {k $$:= v' + v}"
+    by (simp add: fmap_ext)
+  finally show ?thesis .
+qed
+
+lemma inter_plus_addition_notin: (* TODO: Find nicer proofs for SMT calls. *)
+  assumes "m\<^sub>1 $$ k = None"
+  and "m\<^sub>2 $$ k = None"
+  shows "m\<^sub>1(k $$:= v) \<inter>\<^sub>+ m\<^sub>2 = (m\<^sub>1 \<inter>\<^sub>+ m\<^sub>2)"
+proof -
+  from \<open>m\<^sub>2 $$ k = None\<close>
+  have "m\<^sub>1(k $$:= v) \<inter>\<^sub>+ m\<^sub>2 = fmmap_keys (\<lambda>k' v'. v' + m\<^sub>1(k $$:= v) $$! k') (fmdom' m\<^sub>1 \<lhd> m\<^sub>2)"
+    by (smt fmdom'_fmupd fmdom'_notI fmfilter_cong' insert_iff)
+  also have "\<dots> = fmmap_keys (\<lambda>k' v'. v' + m\<^sub>1 $$! k') (fmdom' m\<^sub>1 \<lhd> m\<^sub>2)"
+  proof (intro fmap_ext)
+    fix k'
+    from \<open>m\<^sub>1 $$ k = None\<close>
+    show "fmmap_keys (\<lambda>k' v'. v' + m\<^sub>1(k $$:= v) $$! k') (fmdom' m\<^sub>1 \<lhd> m\<^sub>2) $$ k' =
+      fmmap_keys (\<lambda>k' v'. v' + m\<^sub>1 $$! k') (fmdom' m\<^sub>1 \<lhd> m\<^sub>2) $$ k'"
+      by (smt domIff dom_fmlookup fmdiff_fmupd fmlookup_filter fmlookup_fmmap_keys
+          map_option_is_None option.expand option.map_sel)
+  qed
+  finally show ?thesis .
+qed
+
+lemma union_plus_addition_notin: (* TODO: Find nicer proofs for SMT calls. *)
+  assumes "m\<^sub>1 $$ k = None"
+  and "m\<^sub>2 $$ k = None"
+  shows "m\<^sub>1(k $$:= v) \<union>\<^sub>+ m\<^sub>2 = (m\<^sub>1 \<union>\<^sub>+ m\<^sub>2) ++\<^sub>f {k $$:= v}"
+proof -
+  from \<open>m\<^sub>2 $$ k = None\<close> have "m\<^sub>1(k $$:= v) \<union>\<^sub>+ m\<^sub>2 =
+    fmdom' m\<^sub>2 \<lhd>/ m\<^sub>1 ++\<^sub>f {k $$:= v} ++\<^sub>f fmdom' m\<^sub>1(k $$:= v) \<lhd>/ m\<^sub>2 ++\<^sub>f (m\<^sub>1(k $$:= v) \<inter>\<^sub>+ m\<^sub>2)"
+    by (simp add: fmdom'_notI)
+  also from assms have "\<dots> =
+    fmdom' m\<^sub>2 \<lhd>/ m\<^sub>1 ++\<^sub>f {k $$:= v} ++\<^sub>f fmdom' m\<^sub>1 \<lhd>/ m\<^sub>2 ++\<^sub>f (m\<^sub>1(k $$:= v) \<inter>\<^sub>+ m\<^sub>2)"
+    by (smt fmdom'_fmupd fmfilter_cong insert_iff option.distinct(1))
+  also from assms have "\<dots> = fmdom' m\<^sub>2 \<lhd>/ m\<^sub>1 ++\<^sub>f {k $$:= v} ++\<^sub>f fmdom' m\<^sub>1 \<lhd>/ m\<^sub>2 ++\<^sub>f (m\<^sub>1 \<inter>\<^sub>+ m\<^sub>2)"
+    using inter_plus_addition_notin by metis
+  also from assms have "\<dots> = fmdom' m\<^sub>2 \<lhd>/ m\<^sub>1 ++\<^sub>f fmdom' m\<^sub>1 \<lhd>/ m\<^sub>2 ++\<^sub>f (m\<^sub>1 \<inter>\<^sub>+ m\<^sub>2) ++\<^sub>f {k $$:= v}"
+    using fmap_singleton_comm
+    by (smt fmadd_assoc fmfilter_fmmap_keys fmlookup_filter fmlookup_fmmap_keys)
+  finally show ?thesis .
 qed
 
 end
