Isabelle/Shelley/Ledger.thy
@@ -1,0 +1,11 @@
+section \<open> Ledger State Transition \<close>
+
+theory Ledger
+  imports UTxO Delegation
+begin
+
+text \<open> Ledger state \<close>
+
+type_synonym l_state = "utxo_state \<times> d_p_state"
+
+end
