Isabelle/Shelley/Protocol_Parameters.thy
@@ -1,7 +1,7 @@
 section \<open> Protocol Parameters \<close>
 
 theory Protocol_Parameters
-  imports Finite_Map_Extras
+  imports "HOL.Complex" Finite_Map_Extras
 begin
 
 text \<open> Protocol parameter name \<close>
@@ -15,5 +15,17 @@ typedecl pvalue \<comment> \<open>NOTE: Abstract for now\<close>
 text \<open> Protocol parameter map \<close>
 
 type_synonym p_params = "(ppm, pvalue) fmap"
+
+text \<open> Accessor Functions \<close>
+
+consts tau :: "p_params \<Rightarrow> real" \<comment> \<open>[0, 1]\<close>
+
+consts rho :: "p_params \<Rightarrow> real" \<comment> \<open>[0, 1]\<close>
+
+consts active_slot_coeff :: "p_params \<Rightarrow> real" \<comment> \<open>[0, 1]\<close>
+
+text \<open> Global Constants \<close>
+
+consts slots_per_epoch :: nat
 
 end
